src/robot.lean
@@ -1,0 +1,106 @@
+/- I'm going to define my own wrapper monad around `tactic`. 
+Maybe this is a bad idea. But it will give me practice with typeclasses in Lean so it won't be a waste of time -/
+
+import meta.expr
+import exprset
+open tactic expr
+universe u
+
+namespace robot
+
+meta inductive hyp_telescope
+-- prev are values that have been substituted for the binder in the past.
+|Take  (type : expr) (prev : exprset) (rest : hyp_telescope)
+|Give  (type : expr) (rest : hyp_telescope)
+|Premiss (prop: expr) (rest : hyp_telescope) 
+|Conclusion (prop : expr)
+
+meta structure hyp :=
+    (body : expr) -- the proof term for the hyp
+    (type : hyp_telescope) -- the type has been 'preunwound' to make the conclusion more accessible.
+    (vuln : bool) -- if it's vulnerable, it's fair game for delete_dangling and delete_unmatchable
+    (refs : exprset) -- a table of local_consts that the type depends on.
+
+meta inductive bullet_type |Diamond | Circle
+
+meta structure bullet :=
+    (dependent : exprset)
+    (independent : exprset)
+    (type : bullet_type)
+
+meta def hyps := rbmap expr hyp
+meta structure robot_state :=
+    (vars : list expr)
+    (hyps : hyps)
+    (target : expr)
+    (bullets : rbmap expr bullet)
+
+-- Note that this is just `StateT robot_state tactic α` if we loved monad transformers.
+-- The idea is that `robot` wraps `tactic` to ensure that the extra state remains up to date with the underlying goal structure.
+@[reducible] meta def robot (α : Type u) := robot_state -> tactic (α × robot_state)
+
+meta instance : monad robot :=
+{ map := λ α β f x s, x s >>= (λ ⟨a,s⟩, pure ⟨f a, s⟩)
+, pure := λ α a s, pure ⟨a,s⟩
+, bind := λ α β x f s, x s >>= λ ⟨a,s⟩, f a s
+}
+
+meta instance : alternative robot :=
+{ failure := λ α (s : robot_state), failure 
+, orelse := λ α a b s, (a s : tactic _) <|> (b s)
+}
+
+
+private meta def mk_hyp_telescope : expr -> tactic hyp_telescope
+| (pi n bi a b) := do
+    -- TODO; if `a` is a sigma or a product, convert to a Pi using Exists.elim
+    p <- is_prop a,
+    rest <- mk_hyp_telescope b,
+    return $ if p then hyp_telescope.Take a exprset.empty rest
+            else hyp_telescope.Premiss a rest
+| (app (app `(Exists) a) p) := do
+    p <- whnf p,
+    match p with
+    |(pi n bi _ b) := do
+        rest  <- mk_hyp_telescope b,
+        return $ hyp_telescope.Give a rest
+    |_ := none
+    end
+| x := return $ hyp_telescope.Conclusion x 
+
+private meta def mk_hp_vars_and_hyps : (list expr) -> hyps -> (list expr) -> tactic ((list expr) × hyps)
+|(vs) (hs) ([]) := return ⟨vs, hs⟩
+|(vs) (hs) (v :: t) := do
+    -- TODO expand the definition of the type once?
+    type <- infer_type v,
+    isProp <- is_prop type,
+    if (isProp) then do
+        refs <- return $ from_list $ expr.list_local_const $ type,
+        telescope <- mk_hyp_telescope type,
+        hyp <- return $ hyp.mk v telescope false refs,
+        mk_hp_vars_and_hyps vs (rbmap.insert hs v hyp) t 
+    else mk_hp_vars_and_hyps (v :: vs) hs t
+
+private meta def mk_robot_state : tactic robot_state := do
+    ctx <- local_context,
+    t <- target,
+    ⟨vs, hs⟩ <- mk_hp_vars_and_hyps [] (mk_rbmap _ _) ctx,
+    return $ {vars := vs, hyps := hs, target := t, bullets := mk_rbmap _ _ }
+
+meta def get_hyps : robot $ hyps := λ s, pure ⟨s.hyps, s⟩
+meta def set_hyps : hyps -> robot unit := λ hs s, pure ⟨(), {hyps := hs, ..s}⟩
+meta def get_vars : robot $ list expr := λ s, pure ⟨s.vars, s⟩
+private meta def from_tactic {α : Type} : tactic α -> robot α := λ t s, t >>= λ a, pure ⟨a,s⟩
+meta instance {α : Type} : has_coe (tactic α) (robot α) := ⟨from_tactic⟩ 
+meta def run {α : Type} (r : robot α) : tactic α := prod.fst <$> (mk_robot_state >>= r)
+
+/--Remove a hypothesis. -/
+meta def clear_hyp (e : expr) : robot unit := do
+    hs <- get_hyps,
+    hs' <- pure $ rbmap (λ (h: hyp), e ≠ h.body) hs,
+    clear e,
+    set_hyps hs'
+
+    
+
+end robot
